examples/crypto/dh_hye/HyE.DH.fst
@@ -30,17 +30,17 @@ assume val dh_gen_key: unit -> St (dh_share*dh_exponent)
 type keysize = aeadKeySize AES_128_GCM
 type aes_key = lbytes keysize (* = b:bytes{B.length b = keysize} *)
 
-type log_t (i:id) (r:rid) = m_rref r (seq (PlainDH.key*i:ae_id{b2t (ae_honest i)}*dh_share)) grows
+type log_t (i:id) (r:rid) = m_rref r (seq (entry:(PlainDH.key*dh_share){fst (AE.get_index (fst entry)) = i})) grows
 
 noeq type dh_pkey = 
   | DH_pkey:  #pk_i:id -> #region:rid ->rawpk:dh_share -> log:log_t pk_i region -> dh_pkey
 
 
 noeq abstract type dh_skey =
-  | DH_skey: #sk_i:id -> rawsk:dh_exponent -> pk:dh_pkey -> dh_skey 
+  | DH_skey: #sk_i:id -> rawsk:dh_exponent -> pk:dh_pkey{pk.pk_i=sk_i} -> dh_skey 
 
-val getIndex: dh_skey -> Tot(id)
-let getIndex k = k.sk_i
+val get_index: dh_skey -> Tot(id)
+let get_index k = k.sk_i
 
 val keygen: #i:id -> (parent:rid) -> ST (dh_pair:(k:dh_pkey{k.pk_i=i}) * (k:dh_skey{k.sk_i=i}))
   (requires (fun h -> True))
@@ -74,7 +74,7 @@ type safe_log_append pk entry h0 h1 =
 *)
 val prf_odh_snd: sk:dh_skey -> pk:dh_pkey -> ST (PlainDH.key)
   ( requires (fun _ -> True))
-  ( ensures (fun _ k _ -> HyE.AE.getIndex k = (pk.pk_i, sk.sk_i)
+  ( ensures (fun _ k _ -> HyE.AE.get_index k = (pk.pk_i, sk.sk_i)
   ))
 let prf_odh_snd dh_snd_sk dh_rcv_pk =
   let pk_id = dh_rcv_pk.pk_i in
@@ -82,27 +82,31 @@ let prf_odh_snd dh_snd_sk dh_rcv_pk =
   let i = pk_id, sk_id in
   if ae_honest i && prf_odh then
     let k' = PlainDH.keygen i dh_rcv_pk.region in
-    write_at_end dh_rcv_pk.log (k',i,dh_snd_sk.pk.rawpk);
+    write_at_end dh_rcv_pk.log (k',dh_snd_sk.pk.rawpk);
     k'
   else
     let real_k = dh_exponentiate dh_rcv_pk.rawpk dh_snd_sk.rawsk in
     let k=PlainDH.coerce_key i dh_rcv_pk.region real_k in
     k
 
+val equal_share: dh_sh:dh_share -> entry:(PlainDH.key*dh_share) -> Tot bool
+let equal_share dh_sh entry =
+  snd entry = dh_sh
 
-val prf_odh_rcv: #(sk_id:id) -> dh_share -> dh_skey -> St (ae_id*PlainDH.key)
+
+val prf_odh_rcv: #(sk_id:id) -> dh_sh:dh_share -> dh_sk:dh_skey -> St (k:PlainDH.key)//{fst (AE.get_index k) = sk_id})
 let prf_odh_rcv #sk_id dh_sh dh_rcv_sk =
   if honest sk_id && prf_odh then
     let log = m_read dh_rcv_sk.pk.log in
-    let entry = seq_find (fun (k,i,dh_pk) -> dh_pk=dh_sh) log in
+    let entry = seq_find (equal_share dh_sh) log in
     match entry with
-    | Some (k',i,_) -> i,k'
+    | Some (k',_) -> k'
     | None -> 
-      let i = (dishonestId()), sk_id in
+      let i = sk_id,dishonestId() in
       let raw_k = dh_exponentiate dh_sh dh_rcv_sk.rawsk in
-      i, PlainDH.coerce_key i dh_rcv_sk.pk.region raw_k
+      PlainDH.coerce_key i dh_rcv_sk.pk.region raw_k
   else
     let dis_id = dishonestId() in
-    let i = dis_id, sk_id in
+    let i =  sk_id,dis_id in
     let raw_k = dh_exponentiate dh_sh dh_rcv_sk.rawsk in
-    i,PlainDH.coerce_key i dh_rcv_sk.pk.region raw_k
+    PlainDH.coerce_key i dh_rcv_sk.pk.region raw_k
