examples/crypto/dh_hye/HyE.PlainHPKE.fst
@@ -11,19 +11,25 @@ open FStar.Monotonic.RRef
 open Platform.Bytes
 
 
-abstract type protected_hpke_plain (i:id) = bytes 
+abstract type protected_hpke_plain = 
+  | Prot_hpke_p: #i:ae_id -> b:bytes -> protected_hpke_plain
 //assume Plain_hasEq: hasEq protected_hpke_plain
-type hpke_plain (i:id) = bytes
+type hpke_plain = bytes
+
+val get_index: p:protected_hpke_plain -> Tot (i:ae_id{i=p.i})
+let get_index p =
+  p.i
 
 (* two pure functions, never called when ideal *)
-val repr: #i:id -> p:protected_hpke_plain i{not hpke_ind_cca || not (honest i)} -> Tot (hpke_plain i)
-let repr #i p = p
+val repr: p:protected_hpke_plain{not hpke_ind_cca || not (ae_honest p.i)} -> Tot hpke_plain
+let repr p = p.b
 
 // Change this if we want to use signcryption with hpke_int-ctxt
-val coerce: #i:id -> p:hpke_plain i{not hpke_ind_cca || not (honest i)} -> Tot (protected_hpke_plain i)
-let coerce #i p = p  
+val coerce: #i:ae_id -> p:hpke_plain{not hpke_ind_cca || not (ae_honest i)} -> Tot protected_hpke_plain
+let coerce #i p = 
+  Prot_hpke_p #i p  
 
-val length: #i:id -> protected_hpke_plain i -> Tot nat
-let length #i p = length p
+val length: #i:ae_id -> protected_hpke_plain -> Tot nat
+let length #i p = length p.b
 
 // Create coece_keyshare function
